LeanFunge/Examples.lean
@@ -4,6 +4,8 @@ Released under Apache 2.0 license as described in the file LICENSE.
 Authors: Bangyen Pham
 -/
 import LeanFunge.Examples.Arithmetic
+import LeanFunge.Examples.Countdown
+import LeanFunge.Examples.Factorial
 import LeanFunge.Examples.HelloWorld
 import LeanFunge.Examples.PutGet
 import LeanFunge.Examples.Trampoline
